update hoare.v

Coq/Software Foundation/Q_hoare.v
@@ -3,7 +3,7 @@
   1. Assertion
     - Open Scope XX
   2. Hoare Triples
-  3.
+  3. Proof Rules (& eapply, eassumption )
   4.
   5.
 *)
@@ -75,7 +75,7 @@ context.
 *)
 
 Notation "P <<->> Q" :=
-  (P ->> Q ∧ Q <<- P) (at level 80) : hoare_spec_scope.
+  (P ->> Q /\ Q ->> P) (at level 80) : hoare_spec_scope.
 
 
 
@@ -89,6 +89,270 @@ Notation "P <<->> Q" :=
 
 (* Hoare Triples *)
 (*------------------------------------------------------------*)
+(*
+If command c is started in a state satisfying assertion P, and if 
+c eventually terminates in some final state, then this final 
+state will satisfy the assertion Q.
+Such a claim is called a Hoare Triple.
+*)
+
+Definition hoare_triple
+           (P:Assertion) (c:com) (Q:Assertion) : Prop :=
+  forall st st',
+     c / st \\ st' ->
+     P st ->
+     Q st'.
+
+Notation "{{ P }} c {{ Q }}" :=
+  (hoare_triple P c Q) (at level 90, c at next level)
+  : hoare_spec_scope.
+
+
+(*exercise*)
+Theorem hoare_post_true : forall (P Q : Assertion) c,
+  (forall st, Q st) ->
+  {{P}} c {{Q}}.
+Proof.
+  intros.
+  unfold hoare_triple.
+  intros. apply H.
+Qed.
+
+Theorem hoare_pre_false : forall (P Q : Assertion) c,
+  (forall st, ~(P st)) ->
+  {{P}} c {{Q}}.
+Proof.
+  unfold hoare_triple.
+  intros.
+  unfold not in *.
+  apply H in H1.
+  inversion H1.
+Qed.
+
+
+
+
+
+
+
+
+
+
+(* Proof Rules *)
+(*------------------------------------------------------------*)
+(*
+we'll introduce a rule for reasoning about each of the different 
+syntactic forms of commands in Imp. plus a couple of "structural" rules 
+for gluing things together. We will then be able to prove programs 
+correct using these proof rules, without ever unfolding the definition 
+of hoare_triple.
+*)
+
+
+(* Assignment *)
+(*
+ Hoare rule for assignment:
+      {{ P [X |-> a] }} X ::= a {{ Q }}
+Since Q is an arbitrary Coq proposition, we can't directly "edit" its 
+text. Instead, we can achieve the same effect by evaluating Q in an 
+updated state:
+*)
+
+Definition assn_sub (X: id) (a: aexp) P : Assertion :=
+  fun st => P (t_update st X (aeval st a)).
+
+Notation "P [ X |-> a ]" := (assn_sub X a P) (at level 10).
+(*
+assn_sub 实现了把P中的X替换为a的值的效果。
+因为在st中追加了X的值a，这样只要访问X的地方
+都会得到a的值。
+*)
+
+Theorem hoare_asgn : forall Q X a,
+  {{Q [X |-> a]}} (X ::= a) {{Q}}.
+Proof.
+  intros.
+  unfold hoare_triple.
+  intros. unfold assn_sub in *.
+  inversion H. subst. assumption.
+Qed.
+
+
+Example assn_sub_example :
+  {{(fun st => st X = 3) [X |-> ANum 3]}}
+  (X ::= (ANum 3))
+  {{fun st => st X = 3}}.
+Proof.
+  apply hoare_asgn.
+Qed.
+
+Example assn_sub_ex1 :
+  {{ (fun st => st X <= 5) [X |-> (APlus (AId X) (ANum 1))]  }}
+  X ::= (APlus (AId X) (ANum 1))
+  {{ (fun st => st X <= 5) }}.
+Proof.
+  apply hoare_asgn.
+Qed.
+
+Example assn_sub_ex2 :
+  {{ (fun st => 0 <= st X /\ st X <= 5) [X |-> (ANum 3)]  }}
+  X ::= (ANum 3)
+  {{ (fun st => 0 <= st X /\ st X <= 5) }}.
+Proof. apply hoare_asgn. 
+Qed.
+
+(*
+hoare_asgn_fwd rule复杂不方便：
+
+{{fun st ⇒ P st ∧ st X = m}}
+    X ::= a
+{{fun st ⇒ P st' ∧ st X = aeval st' a }}
+(where st' = t_update st X m)
+
+*)
+Theorem hoare_asgn_fwd :
+  (forall {X Y: Type} {f g : X -> Y},
+     (forall(x: X), f x = g x) -> f = g) ->
+  forall m a P,
+
+  {{fun st => P st /\ st X = m}}
+    X ::= a
+  {{fun st => P (t_update st X m) /\ st X = aeval (t_update st X m) a }}.
+Proof.
+  intros. unfold hoare_triple. intros. split.
+  -inversion H0. inversion H1. subst. clear H1.
+   assert (st =  (t_update
+     (t_update st X (aeval st a)) X
+     (st X))).
+   +apply functional_extensionality. intros.
+    Admitted.
+
+
+(*
+第二种forward rule:
+{{fun st ⇒ P st}}
+    X ::= a
+{{fun st ⇒ ∃m, P (t_update st X m) ∧	st X = aeval (t_update st X m) a}}
+*)
+Theorem hoare_asgn_fwd_exists :
+  forall X a P,
+  {{fun st => P st}}
+    X ::= a
+  {{fun st => exists m, P (t_update st X m) /\
+                st X = aeval (t_update st X m) a }}.
+Proof.
+  unfold hoare_triple.
+  intros.
+  inversion H. subst. exists (aeval st (AId X)).
+  split.
+  -assert (st = (t_update
+     (t_update st X (aeval st a)) X
+     (aeval st (AId X)))).
+   +apply functional_extensionality. intros.
+    Admitted.
+
+
+
+
+
+(* Consequence * 3 *)
+
+Theorem hoare_consequence_pre : forall (P P' Q : Assertion) c,
+  {{P'}} c {{Q}} ->
+  P ->> P' ->
+  {{P}} c {{Q}}.
+Proof.
+  intros.
+  unfold hoare_triple in *.
+  unfold assert_implies in *.
+  intros.
+  apply H0 in H2.
+  apply H in H1.
+  -apply H1. -apply H2.
+Qed.
+
+Theorem hoare_consequence_post : forall (P Q Q' : Assertion) c,
+  {{P}} c {{Q'}} ->
+  Q' ->> Q ->
+  {{P}} c {{Q}}.
+Proof.
+  unfold hoare_triple in *.
+  unfold assert_implies in *.
+  intros.
+  apply H in H1.
+  -apply H0 in H1. apply H1.
+  -apply H2.
+Qed.
+
+Theorem hoare_consequence : forall (P P' Q Q' : Assertion) c,
+  {{P'}} c {{Q'}} ->
+  P ->> P' ->
+  Q' ->> Q ->
+  {{P}} c {{Q}}.
+Proof.
+  intros.
+  apply hoare_consequence_pre with P'.
+  -apply hoare_consequence_post with Q'.
+   +assumption.
+   +assumption.
+  -assumption.
+Qed.
+
+
+Example hoare_asgn_example1 :
+  {{fun st => True}} (X ::= (ANum 1)) {{fun st => st X = 1}}.
+Proof.
+  apply hoare_consequence_pre with 
+    (P':=((fun st : state => st X = 1) [X |-> (ANum 1)])).
+  -apply hoare_asgn.
+  -unfold assn_sub. unfold t_update. simpl. unfold assert_implies.
+   intros. reflexivity.
+Qed.
+
+
+
+
+
+
+
+
+
+
+(* eapply, eassumption *)
+(*------------------------------------------------------------*)
+(*
+每次使用apply时需要手动用with指定元变量的具体值, This is annoying, both 
+because the assertion is a bit long and also because, in 
+hoare_asgn_example1, the very next thing we are going to do — 
+applying the hoare_asgn rule — will tell us exactly what it should 
+be! We can use eapply instead of apply to tell Coq, essentially, "Be 
+patient: The missing part is going to be filled in later in the 
+proof."
+*)
+Example hoare_asgn_example1' :
+  {{fun st => True}}
+  (X ::= (ANum 1))
+  {{fun st => st X = 1}}.
+Proof.
+  eapply hoare_consequence_pre.
+  apply hoare_asgn.
+  unfold assert_implies, assn_sub, t_update. intros. reflexivity.
+Qed.
+
+
+(*
+Coq also provides an eassumption tactic that solves the goal if one 
+of the premises matches the goal up to instantiations of existential 
+variables.
+*)
+Lemma silly2_eassumption : forall (P : nat -> nat -> Prop) 
+                                  (Q : nat -> Prop),
+  (exists y, P 42 y) ->
+  (forall x y : nat, P x y -> Q x) ->
+  Q 42.
+Proof.
+  intros P Q HP HQ. destruct HP as [y HP']. eapply HQ. eassumption.
+Qed.
 
 
 
@@ -102,8 +366,64 @@ Notation "P <<->> Q" :=
 
 
 
+(* SKIP *)
+(*------------------------------------------------------------*)
+Theorem hoare_skip : forall P,
+     {{P}} SKIP {{P}}.
+Proof.
+  unfold hoare_triple. intros.
+  inversion H. subst. assumption.
+Qed.
 
 
+
+
+
+
+
+
+
+
+
+
+
+(* Sequencing *)
+(*------------------------------------------------------------*)
+Theorem hoare_seq : forall P Q R c1 c2,
+     {{Q}} c2 {{R}} ->
+     {{P}} c1 {{Q}} ->
+     {{P}} c1;;c2 {{R}}.
+Proof.
+  unfold hoare_triple.
+  intros.
+  inversion H1. subst.
+  apply H0 in H5. apply H in H8.
+  -assumption. -assumption. -assumption.
+Qed.
+
+(*
+in the rule hoare_seq, the premises are given in backwards order (c2 
+before c1). This matches the natural flow of information in many of 
+the situations, since the natural way to construct a Hoare-logic 
+proof is to begin at the end of the program (with the final 
+postcondition) and push postconditions backwards through commands 
+until we reach the beginning.
+*)
+
+
+Example hoare_asgn_example3 : forall a n,
+  {{fun st => aeval st a = n}}
+  (X ::= a;; SKIP)
+  {{fun st => st X = n}}.
+Proof.
+  intros.
+  eapply hoare_seq.
+  -apply hoare_skip.
+  -eapply hoare_consequence_pre.
+   +apply hoare_asgn.
+   +unfold assert_implies, assn_sub. intros.
+    assumption.
+Qed.
 
 
 
